thys/MFODL_Monitor_Devel/Formula.thy
@@ -1220,6 +1220,10 @@ lemma future_bounded_get_and:
   by (induction \<phi>) simp_all
 
 lemma safe_letprev_convert_multiway: "safe_letprev p b \<phi> \<Longrightarrow> safe_letprev p b (convert_multiway \<phi>)"
+  apply (induction p b \<phi> rule: safe_letprev.induct)
+                   apply simp_all
+   apply safe
+  sledgehammer
   sorry (*by (induction p b \<phi> rule: safe_letprev.induct)(simp_all)*) (*TODO*)
 
 lemma safe_convert_multiway: "safe_formula \<phi> \<Longrightarrow> safe_formula (convert_multiway \<phi>)"
